Session.v
@@ -4,6 +4,8 @@ Require Import Arith.
 Require Import Eqdep_dec.
 Require Import Coq.Logic.FunctionalExtensionality.
 Require Import CpdtTactics.
+Add LoadPath "/Users/adampetz/Documents/Fall_2015_Courses/armored/session/protosynth".
+Require Import ProtocolSynthesis4.
 
 Inductive protoType : Type :=
 | Send : type -> protoType -> protoType
@@ -12,6 +14,28 @@ Inductive protoType : Type :=
 | Offer : protoType -> protoType -> protoType  
 | Eps : type -> protoType.
 
+(*
+Section mSection.
+  
+Axiom networkReceive : nat -> Message.
+
+Fixpoint sessionToProtoExp (s:Session) (n:nat) : (type * protoType).
+Proof.
+  intros. 
+  destruct s eqn : mm.
+  exact (Basic, snd (sessionToProtoExp s0 (S n))).
+  specialize (networkReceive n). intros.
+  destruct H eqn : mmm.
+  exact (Basic, snd (sessionToProtoExp (s0 m))).
+  exact (Basic, (Eps Basic)).
+Defined.  Check sessionToProtoExp.
+
+
+End mSection.
+
+Check sessionToProtoExp.
+*)
+                                                  
 Inductive protoExp : type -> protoType -> Type :=
 | SendC {t:type} {T:type} {p':protoType}  : (message t) -> (protoExp T p')
     -> protoExp T (Send t p')
@@ -20,15 +44,6 @@ Inductive protoExp : type -> protoType -> Type :=
     -> (protoExp (if(b) then R else S) (Choice r s))
 | OfferC {r s : protoType} {R S:type} : (protoExp R r) -> (protoExp S s)
                                         -> (protoExp (Either R S) (Offer r s))| ReturnC {t:type} : (message t) -> protoExp t (Eps t).
-
-(*
-Inductive DualR' : forall (T T':type), forall (t t':protoType), (protoExp T t) -> (protoExp T' t') -> Prop :=
-
-| returnR' : forall T T' r1 r2, DualR' T T' (Eps T) (Eps T') r1 r2
-| sendR' : forall T T' t' t'' x y r1 r2 r3 r4,
-    (T = T') ->
-    DualR' x y t' t'' r3 r4 ->
-    DualR' x y (Send T t') (Receive T t'') r1 r2.   *)  
 
 Inductive DualR : forall (T T':type), forall (t t':protoType), (protoExp T t) -> (protoExp T' t') -> Prop :=
 | returnR' : forall T T' (m:message T) (m':message T'),
@@ -142,14 +157,8 @@ Fixpoint DualT (t t':protoType) : Prop :=
     end
   end.
 
-  (*repeat match goal with        
-  (*| [ |- {DualT (?T _ _) (?T _ _)} + {~ DualT (?T _ _) (?T _ _)} ]
-    => right; unfold not; trivial  *)
-  | [ |- _ ] =>  right; unfold not; intros; inversion H; contradiction
-  end. *)
-
 Fixpoint DualT_dec (t t':protoType) : {DualT t t'} + {~ DualT t t'}.
-Proof. 
+Proof.
   destruct t; destruct t';
 
   (* Eliminate all un-interesting cases *)
@@ -167,7 +176,7 @@ Proof.
   destruct (DualT_dec t1 t'1); destruct (DualT_dec t2 t'2);
   try (right; unfold not; intros; inversion H; contradiction);
   try( left; split; assumption)
-    );
+    ).
 
   (* Eps/Eps case *)
   left. simpl. trivial.
@@ -175,35 +184,6 @@ Proof.
 Defined.
 
 Definition Dual {t t':protoType} {T T':type} (p1:protoExp T t) (p2:protoExp T' t') : Prop := DualT t t'.
-
-(*
-Fixpoint ifDualThenDualR {t t':protoType} {T T':type} (n:nat) (p1:protoExp T t) (p2:protoExp T' t') : Dual p1 p2 -> DualR _ _ _ _ p1 p2.
-  refine ( fun H => 
-      match n with
-      | O => _
-      | S n' => _
-      end ). 
-  dependent inversion p1; subst; dependent inversion p2; subst; try inversion H. subst. constructor. apply ifDualThenDualR. exact n'. unfold Dual. assumption. subst. constructor. apply ifDualThenDualR. exact n'. unfold Dual. assumption.
-  destruct b.
-  constructor. apply ifDualThenDualR. exact n'. unfold Dual. assumption. apply ifDualThenDualR. exact n'. unfold Dual. assumption.
-  constructor. apply ifDualThenDualR. exact n'. unfold Dual. assumption. apply ifDualThenDualR. exact n'. unfold Dual. assumption.
-  destruct b.
-    constructor. apply ifDualThenDualR. exact n'. unfold Dual. assumption. apply ifDualThenDualR. exact n'. unfold Dual. assumption.
-    constructor. apply ifDualThenDualR. exact n'. unfold Dual. assumption. apply ifDualThenDualR. exact n'. unfold Dual. assumption.
-    constructor. 
-Abort. 
-  
-  
-
-
-  try inversion H. dependent induction p
-
-  
-  apply ifDualThenDualR. apply H. apply ifDualThenDualR. apply H. apply ifDualThenDualR. apply H. apply ifDualThenDualR. apply H. constructor. Defined.
-  
-
-  
-Abort. *)
 
 Theorem ifDualThenDualR {t t':protoType} {T T':type} : forall (p1:protoExp T t) (p2:protoExp T' t'), Dual p1 p2 -> DualR _ _ _ _ p1 p2.
 Proof.
@@ -224,89 +204,8 @@ Proof.
   apply IHp1_2. unfold Dual. assumption.
   constructor. subst. apply IHp1_1. unfold Dual. assumption.
   apply IHp1_2. unfold Dual. assumption.
-  constructor. Qed.
-
-
-  (*
-  f0 : message t0 -> protoExp T p'
-  H10 : t0 = t0
-  H4 : DualR T T0 p' p'0 (f0 m) p2
-             p : message t0 -> protoExp T p' 
-  H : forall (m : message t0) (T' : type) (t' : protoType)
-        (p2 : protoExp T' t'), DualR T T' p' t' (p m) p2 -> Dual (p m) p2
-   *)
-
-Definition sameExpType {T T':type} {p p':protoType} (a:protoExp T p) (b:protoExp T' p') : Prop := p = p' /\ T = T'.
-
-(* x : DualR X Y' p' p'0 a (p m0)  *)
-Lemma poopypants : forall T x y p1 p2 a p (m0 m:message T), DualR x y p1 p2 a (p m0) -> DualR x y p1 p2 a (p m).
-Proof.
-  Abort.
-
-    
-Lemma sameTypeDualR {T T' p2T:type} {p p' p2t:protoType} : forall  (b:protoExp T' p') (a:protoExp T p) p2, (sameExpType a b) -> (DualR _ p2T _ p2t a p2) -> (DualR _ _ _ _ b p2).
-Proof.
-  intros b a p2 same aDual.
-  inversion same; subst.
-  induction b. dep_destruct a. dep_destruct p2. generalize dependent m.  inversion aDual. dep_destruct aDual.  (*apply poopypants with (m:=m) in x0. constructor. *)
-
-Abort.
-
-(*rewrite H9.
-
-
-
-
-
-
-
-
-
-
-
-
-
-
-
-
-
-
-
-
-
-  
-  admit.                                                   
-  inversion H1.
-  inversion H1.
-  inversion H1.
-  inversion H1.
-  inversion H2.
-  admit.
-  inversion H2.
-  inversion H2.
-  inversion H2.
-  inversion H.
-  inversion H.
-  inversion H.
-  inversion H.
-  admit.
-  inversion H.
-  inversion H.
-  inversion H.
-  inversion H.
-  inversion H.
-  inversion H.
-  inversion H.
-  admit.
-  inversion H.
-  inversion H.
-  inversion H.
-  inversion H.
-  inversion H.
-  inversion H.
-  inversion H.
-  constructor. *)
-
+  constructor.
+Qed.
                                        
 Theorem ifDualRthenDual {t t':protoType} {T T':type} : forall (p1:protoExp T t) (p2:protoExp T' t'), DualR _ _ _ _ p1 p2 -> Dual p1 p2.
 Proof.
@@ -321,44 +220,10 @@ Proof.
   try (intro xx; inversion xx; contradiction).
   try (intro xx; inversion xx; contradiction).
 
-  (*intro. unfold Dual. inversion H0. subst. simpl_existTs. subst. split.  assumption. *)
-   (*apply (H _ _ _ _ H4). *)
-
-  
-  (*generalize dependent p.*) generalize dependent t. generalize dependent T.  destruct p2.
-  intros. unfold Dual. dep_destruct H0. (*simpl_existTs; subst. *) 
+  generalize dependent t. generalize dependent T.  destruct p2.
+  intros. unfold Dual. dep_destruct H0. 
   split. reflexivity. unfold Dual in H. apply (H m _ p'0 p2 x).
 
-  (*
-  assert (DualR T T0 p' p'0 (p m) p2). Print sameTypeDualR. apply (sameTypeDualR (f0 m) (p m)). unfold sameExpType. reflexivity. assumption. apply (H m T0 p'0 p2 H1).
-
-  admit. apply (H _ _ _ p2 H4).
-
-  inversion H0. simpl_existTs. rewrite H12 in H4. apply IHp2.
-  admit.
-
-
-                          apply inj_pairT2 in H8. apply inj_pairT2 in H8. apply inj_pairT2 in H8
-  simpl_existTs split. reflexivity.
-
-  generalize dependent p. dependent inversion p2.
-  intro. inversion H2. simpl_existTs. assert (protoExp T p'). exact (f0 m1). assert (X0 = (f m1)). subst.
-  
-  
-
-  unfold Dual. simpl. inversion H0. simpl_existTs. split. assumption. subst. unfold Dual in H. apply (H _ _ _ p2 H4).
-
-  apply (H _ _ _ p2 H4).
-  
-  try (intro xx; inversion xx; contradiction)
-  intro. unfold Dual in H. unfold Dual. simpl. split. inversion H0. simpl_existTs.  subst. assumption. inversion H0. simpl_existTs. subst. assert (protoExp T p'). exact (p m). unfold Dual in IHp2.
-
-  apply (H _ _ _ p2 H4).
-
-      apply f0 in m. subst apply (H _ _ _ _ H6).
-  split. assumption.
-  simpl_existTs.
-  *)
   intro aa. inversion aa.
   intro aa. inversion aa.
   intro aa. inversion aa.
@@ -383,25 +248,26 @@ Proof.
      intro aa. inversion aa.
      intro aa. inversion aa.
      intro. unfold Dual. simpl. trivial.
+Qed.
 
 Fixpoint runProto' {t t':protoType} {T T':type} (p1:protoExp T t) (p2:protoExp T' t') 
   : (Dual p1 p2) -> (message T).
 Proof.
 
-  intros; destruct p1; destruct p2; try inversion H.
+       intro pf. destruct p1 (*eqn : p1Val*); destruct p2 (*eqn : p2Val*); try (inversion pf).
 
-       subst. apply (runProto' _ _ _ _ p1 (p m) (*l*)(*(protoExpLength (p m))*)). assumption.
-       subst. apply (runProto' _ _ _ _ (p m) p2 ). assumption.
+       subst. apply (runProto' _ _ _ _ p1 (p m)). unfold Dual. assumption.
+       subst. apply (runProto' _ _ _ _ (p m) p2). unfold Dual. assumption.
 
        destruct b.
-       apply (runProto' _ _ _ _ p1_1 p2_1 ). assumption.
-       apply (runProto' _ _ _ _ p1_2 p2_2 ). assumption.
+       apply (runProto' _ _ _ _ p1_1 p2_1 ). unfold Dual. assumption.
+       apply (runProto' _ _ _ _ p1_2 p2_2 ). unfold Dual. assumption.
        
        destruct b.
        assert (message R).
-       apply (runProto' _ _ _ _ p1_1 p2_1 ). assumption. exact (leither _ _ X).
+       apply (runProto' _ _ _ _ p1_1 p2_1 ). unfold Dual. assumption. exact (leither _ _ X).
        assert (message S).
-       apply (runProto' _ _ _ _ p1_2 p2_2 ). assumption. exact (reither _ _ X).
+       apply (runProto' _ _ _ _ p1_2 p2_2 ). unfold Dual. assumption. exact (reither _ _ X).
 
        exact m.
 Defined.
@@ -432,79 +298,65 @@ Definition runProto {t t':protoType} {T T':type} (p1:protoExp T t) (p2:protoExp 
 
 Definition nextType{T T':type} {t t':protoType} (p1:protoExp T t) (p2:protoExp T' t') : (Dual p1 p2) -> protoType.
   intros; destruct p1; destruct p2; try inversion H. exact p'. exact p'. destruct b. exact r. exact s. destruct b. exact r. exact s. exact (Eps t0).
-Defined.
+Defined. Print nextType.
+
+Definition recFunNextpType {t T:type} {p':protoType} (p: (message t) -> (protoExp T p')) : protoType := p'.
+
+Definition recFunNextType {t T:type} {p':protoType} (p: (message t) -> (protoExp T p')) : type := T.
+
+Definition ptOf {T:type} {t:protoType} (p1:protoExp T t) : protoType := t.
+Definition tOf {T:type} {t:protoType} (p1:protoExp T t) : type := T.
+Definition mType {t:type} (m:message t) : type := t.
+
+Definition nextType'{T T':type} {t t':protoType} (p1:protoExp T t) (p2:protoExp T' t') : protoType :=
+  match p1 with
+  | SendC _ p' => ptOf p'
+  | ReceiveC p => recFunNextpType p
+  | ChoiceC b p1' p1'' =>
+    match p2 with
+    | OfferC _ _ => if b then ptOf p1' else ptOf p1''   
+    | _ => Eps Basic
+    end
+  | OfferC p1' p1'' =>
+    match p2 with
+    | ChoiceC b _ _ => if b then ptOf p1' else ptOf p1''
+    | _ => Eps Basic
+    end
+  | ReturnC m => Eps (mType m)
+  end.
 
 Definition nextRtype {T T':type} {t t':protoType} (p1:protoExp T t) (p2:protoExp T' t') : (Dual p1 p2) -> type.
   intros; destruct p1; destruct p2; try inversion H. exact T. exact T. destruct b. exact R. exact S. destruct b. exact R. exact S. exact t0.
 Defined.
 
-Fixpoint nextRtype' {T T':type} {t t':protoType} (p1:protoExp T t) (p2:protoExp T' t') : type.
-  refine (
+Definition nextRtype' {T T':type} {t t':protoType} (p1:protoExp T t) (p2:protoExp T' t') : type :=
   match p1 with
-  | SendC _ _ =>
+  | SendC _ p' => tOf p'
+  | ReceiveC p => recFunNextType p
+  | ChoiceC b p1' p1'' => match p2 with
+    | OfferC _ _ => if b then tOf p1' else tOf p1''
+    | _ => Basic
+    end
+  | OfferC p1' p1'' =>
     match p2 with
-    | ReceiveC f => _ 
-    | _ => _
+    | ChoiceC b _ _ => if b then tOf p1' else tOf p1''
+    | _ => Basic
     end
-  | ReceiveC _ =>
-    match p2 with
-    | SendC _ _ => _                            
-    | _ => _
-    end
-  | ChoiceC b _ _ => match p2 with
-    | OfferC _ _ => _                                                         
-    | _ => _
-    end
-  | OfferC _ _ =>
-    match p2 with
-    | ChoiceC b _ _ => _
-    | _ => _
-    end
-  | ReturnC _ => _
-  end).
-  exact T.
-  destruct (eq_type_dec t0 t2).
-    subst. apply (nextRtype' _ _ _ _ p0 (f m)).
-    exact T.
-  exact T.
-  exact T.
-  exact T.
- 
-  destruct (eq_type_dec t0 t2).
-    subst. apply (nextRtype' _ _ _ _ (p0 m) p4).
-    exact T.
-  exact T.
-  exact T.
-  exact T.
-  exact T.
-
-  exact T.
-  exact T.
-  exact T.
-  destruct b.
-    apply (nextRtype' _ _ _ _ p3 p7).
-    apply (nextRtype' _ _ _ _ p4 p8).
-  exact T.
-    
-  exact T.
-  exact T.
-  destruct b.
-    apply (nextRtype' _ _ _ _ p3 p7).
-    apply (nextRtype' _ _ _ _ p4 p8).  
-  exact T.
-  exact T.
-
-  exact t0.
-Defined.
-
+  | ReturnC m => mType m                            
+  end.
 
 Theorem senRecOnce{t T1 T2:type}{t1 t2:protoType}{p1':protoExp T1 t1} {f : (message t) -> (protoExp T2 t2)} : forall (m:message t),
     (nextRtype' (SendC m p1') (ReceiveC f)) = (nextRtype' p1' (f m)).
 Proof.
-  intros. simpl. Abort.
+  intros. simpl. unfold tOf. unfold nextRtype'. Abort.
+
+Theorem senRecOnce'{t T1 T2:type}{t1 t2:protoType}{p1':protoExp T1 t1} {f : (message t) -> (protoExp T2 t2)} : forall (m:message t),
+    (nextRtype' (SendC m p1') (ReceiveC f)) = T1.
+Proof.
+  intros. simpl. unfold tOf. reflexivity. Qed.
   
 
-Definition runProto'OneStep {t t':protoType} {T T':type} (p1:protoExp T t) (p2:protoExp T' t') (p:Dual p1 p2) : (protoExp (nextRtype p1 p2 p) (nextType p1 p2 p)).
+Definition runProto'OneStep {t t':protoType} {T T':type} (p1:protoExp T t) (p2:protoExp T' t') (p:Dual p1 p2) : (protoExp (nextRtype' p1 p2) (nextType' p1 p2)).
   destruct p1; destruct p2; try inversion p.
 simpl. destruct p. exact p1.
 simpl. destruct p. subst. exact (p0 m).
@@ -514,13 +366,13 @@ simpl. destruct p. exact p1_2.
 destruct b.
 simpl. destruct p. exact p1_1.
 simpl. destruct p. exact p1_2.
-simpl. destruct p. exact (ReturnC m0).
+simpl. destruct p. exact (ReturnC m).
 Defined.
 
-Definition runProtoOneStep {t t':protoType} {T T':type} (p1:protoExp T t) (p2:protoExp T' t') (p:Dual p1 p2) : ((protoExp (nextRtype p1 p2 p) (nextType p1 p2 p)) * (protoExp (nextRtype p2 p1 (DualSymm p)) (nextType p2 p1 (DualSymm p)) )) :=
+Definition runProtoOneStep {t t':protoType} {T T':type} (p1:protoExp T t) (p2:protoExp T' t') (p:Dual p1 p2) : ((protoExp (nextRtype' p1 p2) (nextType' p1 p2)) * (protoExp (nextRtype' p2 p1) (nextType' p2 p1) )) :=
   let x := (runProto'OneStep p1 p2 p) in
   let y := (runProto'OneStep p2 p1 (DualTSymm p)) in
-  (x,y).    
+  (x,y).
 
 Fixpoint runProtoMultiStep' {t t':protoType} {T T':type} (p1:protoExp T t) (p2:protoExp T' t') (n:nat) : (Dual p1 p2) -> (message T * message T').
   refine
@@ -539,16 +391,16 @@ Fixpoint runProtoMultiStep' {t t':protoType} {T T':type} (p1:protoExp T t) (p2:p
     exact (bad (Either R S), bad S0).
   exact (m, m0).
   destruct (runProtoOneStep p1 p2 pf);
-  destruct p1; destruct p2; try inversion pf;
+    destruct p1; destruct p2; try inversion pf;
   try
-  (subst; destruct pf; cbv in p;  cbv in p0;  destruct (runProtoMultiStep' _ _ _ _ p p0 n' d); exact (m0, m1)).
+  (subst; destruct pf; cbv in p;  cbv in p0;  destruct (runProtoMultiStep' _ _ _ _ p p0 n' H0); exact (m0, m1)).
   destruct b.
-  destruct pf. cbv in p. cbv in p0. destruct (runProtoMultiStep' _ _ _ _ p p0 n' d). exact (m, leither _ _ m0).
-  destruct pf. cbv in p. cbv in p0. destruct (runProtoMultiStep' _ _ _ _ p p0 n' d0). exact (m, reither _ _ m0).
+  destruct pf. cbv in p. cbv in p0. destruct (runProtoMultiStep' _ _ _ _ p p0 n' H). exact (m, leither _ _ m0).
+  destruct pf. cbv in p. cbv in p0. destruct (runProtoMultiStep' _ _ _ _ p p0 n' H0). exact (m, reither _ _ m0).
   destruct b.
-    destruct pf. cbv in p. cbv in p0. destruct (runProtoMultiStep' _ _ _ _ p p0 n' d). exact (leither _ _  m, m0).
-    destruct pf. cbv in p. cbv in p0. destruct (runProtoMultiStep' _ _ _ _ p p0 n' d0). exact (reither _ _ m, m0).
-    destruct pf. cbv in p. cbv in p0. assert (Dual p p0). reflexivity. destruct (runProtoMultiStep' _ _ _ _ p p0 n' H). exact (m2, m1). Defined.
+    destruct pf. cbv in p. cbv in p0. destruct (runProtoMultiStep' _ _ _ _ p p0 n' H). exact (leither _ _  m, m0).
+    destruct pf. cbv in p. cbv in p0. destruct (runProtoMultiStep' _ _ _ _ p p0 n' H0). exact (reither _ _ m, m0).
+    destruct pf. cbv in p. cbv in p0. assert (Dual p p0). reflexivity. destruct (runProtoMultiStep' _ _ _ _ p p0 n' H). exact (m1, m2). Defined.
 
 Definition runProtoMultiStep {t t':protoType} {T T':type} (p1:protoExp T t) (p2:protoExp T' t') : (Dual p1 p2) -> (message T * message T') :=
   fun pf =>
@@ -626,55 +478,7 @@ Proof.
   dependent induction p1; dependent induction p2; try (inversion H).
   exists (bad T). inversion H0. clear H4. subst.
   apply sendR. Abort.
-                                                                                        
-(*Fixpoint dualIfR {t t':protoType} {T T':type} (p1:protoExp T t) (p2:protoExp T' t') : (exists m, runProtoR _ _ _ _ p1 p2 m) -> DualR _ _ _ _ p1 p2.
-Proof.
-  intros H. dependent inversion p1. dependent inversion p2.
-  inversion H. subst. inversion H4.
-  inversion H. inversion H4. simpl_existTs. subst. inversion H7. simpl_existTs. subst. inversion H4. simpl_existTs. inversion H3. simpl_existTs. clear H28. clear H3. subst. constructor. dependent inversion p. 
-  inversion H1.
-  inversion H1.
-  inversion H1.
-  inversion H1.
-  admit.
-  inversion H1.
-  admit.
-  inversion H1.
-  constructor.
-  inversion H. subst. inversion H4. simpl_existTs. clear H3. subst. constructor.
-
-
-
-  
-  intros. dependent induction p1; dependent induction p2; try (inversion H); try (inversion H0).
-
-  admit. admit. inversion H1. inversion H2. inversion H1. inversion H1. inversion H1. inversion H1. simpl_existTs. destruct b. constructor. assumption. assumption. subst.
-
-
-
-  dependent inversion H1. simpl_existTs. inversion H5. simpl_existTs. clear H24. clear H5. subst. constructor. dependent inversion p1.
-  
-
-  clear H5. subst. apply sendR'.
-
-  specialize IHp1 with (ReceiveC p). subst. Abort. (*apply IHp1.
-
-  runProtoR T T0 p' p'0 p1' (f0 m1) m'
-  intros. destruct p1; destruct p2. inversion H; inversion H0.
-  split.
-  inversion H0. reflexivity.
-  induction H4. simpl. trivial.
-  simpl.
-  split. reflexivity.
-  subst. inversion H9. Abort. (*
-  apply (IHrunProtoR p1' f m' f).
-  match goal with
-  | [ H : (existT (fun x : type => _) _ _ = existT _ _ _) |- _ ] => inversion H; try subst
-  end
-
-  inversion H0 reflexivity
-  inversion H0. inversion H4. subst. simpl. trivial. inversion H4. subst. simpl. split. trivial. Abort *) *) *)
-
+                                                                             
 Theorem DualIfR {t t':protoType} {T T':type} : forall (p1:protoExp T t) (p2:protoExp T' t') m,
     runProtoR T T' t t' p1 p2 m -> DualR T T' t t' p1 p2.
 Proof.
@@ -723,15 +527,21 @@ Lemma DualInner {t t':protoType} {T T':type} {p1:protoExp T t} {p2:protoExp T' t
 Proof.
 Admitted.
 
+Hint Resolve nextType nextRtype.
 
 Theorem rIfMulti {t t':protoType} {T T':type} : forall (p1:protoExp T t) (p2:protoExp T' t') (pf:Dual p1 p2) m, fst (runProtoMultiStep p1 p2 pf) = m -> runProtoR T T' t t' p1 p2 m.
 Proof.
    intros p1. generalize dependent t'. generalize dependent T'.
    induction p1; dependent inversion p2; try (intros m1 runR; inversion runR; contradiction).
-   intros. inversion pf. subst. constructor. assert (Dual p1 (p m)).
+   intros. inversion pf. subst. constructor. assert (Dual p1 (p m)). admit.
    assert ((runProto'OneStep (send m; p1) (ReceiveC p) pf) = p1).
+   unfold runProto'OneStep. destruct pf. reflexivity.
+   
    apply IHp1 with (pf := H). assert ( (runProtoMultiStep p1 (p m) H) =
-   (runProtoMultiStep (send m; p1) (ReceiveC p) pf) ). apply osEval. rewrite H0. reflexivity.  
+                                       (runProtoMultiStep (send m; p1) (ReceiveC p) pf) ). unfold runProtoMultiStep at 2. assert ((Init.Nat.max (protoExpLength (send m; p1))
+        (protoExpLength (ReceiveC p))) = 1). admit. rewrite H1. inversion pf.  unfold runProtoMultiStep'.  unfold runProtoOneStep. unfold nextRtype'. unfold nextType'. unfold recFunNextType. unfold recFunNextpType. unfold tOf. unfold ptOf. unfold runProto'OneStep. unfold recFunNextType. unfold recFunNextpType. cbv. simpl_eq. 
+
+   apply osEval. rewrite H0. reflexivity.
    intros. inversion pf. subst. constructor. assert (Dual (p m) p0). admit. apply H with (pf := H0). assert ( (runProtoMultiStep (p m) p0 H0) =
    (runProtoMultiStep (ReceiveC p) (send m; p0)  pf) ). apply osEvalFlipped. rewrite H1. reflexivity.
 
@@ -753,7 +563,7 @@ Proof.
 
    assert ((fst (runProtoMultiStep (offer p1_1 p1_2) (choice false p p0) pf)) = (reither R S (fst (runProtoMultiStep p1_2 p0 H3)))). admit. rewrite H. apply offerRf with (m:=(fst (runProtoMultiStep p1_1 p H2))). apply IHp1_1 with (pf:=H2). reflexivity. apply IHp1_2 with (pf:= H3). reflexivity.
 
-   intros. inversion H1. assert ((fst (runProtoMultiStep (ReturnC m) (ReturnC m0) pf)) = m). admit. rewrite H3. constructor. 
+   intros. inversion H1. assert ((fst (runProtoMultiStep (ReturnC m) (ReturnC m0) pf)) = m). admit. rewrite H3. constructor.
    
    
    Check ( (fst (runProtoMultiStep (offer p1_1 p1_2) (choice true p p0) pf))). 
@@ -782,9 +592,6 @@ Proof.
 Theorem multiIfR {t t':protoType} {T T':type} (p1:protoExp T t) (p2:protoExp T' t') (pf:Dual p1 p2) : forall m, runProtoR T T' t t' p1 p2 m -> fst (runProtoMultiStep p1 p2 pf) = m.
 Proof. 
   intros. dep_destruct p1. dep_destruct p2. dep_destruct H. unfold runProtoMultiStep. 
-
-  (*destruct m0; destruct m. destruct n; destruct n0. inversion H. subst.  apply inj_pair2_eq_dec in H11.  apply inj_pair2_eq_dec in H11.  apply inj_pair2_eq_dec in H11.  apply inj_pair2_eq_dec in H12.  apply inj_pair2_eq_dec in H8.  apply inj_pair2_eq_dec in H8.  apply inj_pair2_eq_dec in H7. rewrite <- H11. rewrite <- H8. inversion H3.  apply inj_pair2_eq_dec in H17.  apply inj_pair2_eq_dec in H16.  apply inj_pair2_eq_dec in H14.  subst. inversion H3.  apply inj_pair2_eq_dec in H6.  apply inj_pair2_eq_dec in H4.  apply inj_pair2_eq_dec in H4.  apply inj_pair2_eq_dec in H2.  apply inj_pair2_eq_dec in H2.  apply inj_pair2_eq_dec in H16.  apply inj_pair2_eq_dec in H14. subst.  inversion H3.  apply inj_pair2_eq_dec in H6.  apply inj_pair2_eq_dec in H7.  apply inj_pair2_eq_dec in H7.  apply inj_pair2_eq_dec in H8. subst. cbv. subst. cbv 
-*)
 
 
 
