SessionClean.v
@@ -1,0 +1,364 @@
+Require Export Crypto.
+Require Import Program.
+Require Import Arith.
+Require Import Eqdep_dec.
+Require Import Coq.Logic.FunctionalExtensionality.
+Require Import CpdtTactics.
+
+Inductive protoType : Type :=
+| Send : type -> protoType -> protoType
+| Receive : type -> protoType -> protoType
+| Choice : protoType -> protoType -> protoType
+| Offer : protoType -> protoType -> protoType  
+| Eps : type -> protoType.
+
+Fixpoint returnType (p:protoType) : type :=
+  match p with
+  | Send _ p' => returnType p'
+  | Receive _ p' => returnType p'
+  | _ => Basic
+  end.
+
+                                                  
+Inductive protoExp : type -> protoType -> Type :=
+| SendC {t:type} {T:type} {p':protoType}  : (message t) -> (protoExp T p')
+    -> protoExp T (Send t p')
+| ReceiveC {t:type} {T:type} {p':protoType} : ((message t)->(protoExp T p'))     -> protoExp T  (Receive t p') 
+| ChoiceC (b:bool) {r s:protoType} {R S:type} :(protoExp R r) -> (protoExp S s)
+    -> (protoExp (if(b) then R else S) (Choice r s))
+| OfferC {r s : protoType} {R S:type} : (protoExp R r) -> (protoExp S s)
+                                        -> protoExp (Either R S) (Offer r s)
+| ReturnC {t:type} : (message t) -> protoExp t (Eps t).
+
+
+Definition funType{t T:type}{p':protoType} (f:(message t) -> (protoExp T p')) : type := t.
+
+Notation "x :!: y" := (Send x y)
+                        (at level 50, left associativity). 
+Notation "x :!: y" := (protoExp (Send x y))
+                        (at level 50, left associativity).
+
+Notation "x :?: y" := (Receive x y)
+                        (at level 50, left associativity).  
+Notation "x :?: y" := (protoExp (Receive x y))
+                        (at level 50, left associativity).
+
+Notation "x :+: y" := (Choice x y)
+                        (at level 50, left associativity).
+Notation "x :+: y" := (protoExp (Choice x y))
+                        (at level 50, left associativity).  
+
+Notation "x :&: y" := (Offer x y)
+                        (at level 50, left associativity).
+Notation "x :&: y" := (protoExp (Offer x y))
+                        (at level 50, left associativity). 
+
+Notation "'send' n ; p" := (SendC n p)
+                            (right associativity, at level 60).
+Notation "x <- 'receive' ; p " := (ReceiveC (fun x => p)) 
+                                    (right associativity, at level 60). 
+
+Notation "'offer'" := OfferC.
+
+Notation "'choice'" := ChoiceC.  
+
+Definition EpsC := ReturnC (basic 0).
+
+Fixpoint DualT (t t':protoType) : Prop :=
+  match t with
+  | Send p1T p1' =>
+    match t' with
+    | Receive p2T p2' => (p1T = p2T) /\ (DualT p1' p2')    
+    | _ => False
+    end
+  | Receive p1T p1' =>
+    match t' with
+    | Send p2T p2' => (p1T = p2T) /\ (DualT p1' p2')                                
+    | _ => False
+    end
+  | Choice p1' p1'' =>
+    match t' with
+    | Offer p2' p2'' => (DualT p1' p2') /\ (DualT p1'' p2'')                                                             
+    | _ => False
+    end
+  | Offer p1' p1'' =>
+    match t' with
+    | Choice p2' p2'' => (DualT p1' p2') /\ (DualT p1'' p2'')                                                               
+    | _ => False
+    end
+  | Eps _ =>
+    match t' with
+    | Eps _ => True           
+    | _ => False
+    end
+  end.
+
+Fixpoint DualT_dec (t t':protoType) : {DualT t t'} + {~ DualT t t'}.
+Proof.
+  destruct t; destruct t';
+
+  (* Eliminate all un-interesting cases *)
+  try (right; unfold not; intros; inversion H; contradiction);
+
+  (* For the Send/Receive, Receive/Send cases *)
+  try (
+  destruct (eq_type_dec t t1); destruct (DualT_dec t0 t');
+  try (right; unfold not; intros; inversion H; contradiction);
+  try (left; split; assumption)
+  );
+
+  (* For the Choice/Offer, Offer/Choice cases *)
+  try (
+  destruct (DualT_dec t1 t'1); destruct (DualT_dec t2 t'2);
+  try (right; unfold not; intros; inversion H; contradiction);
+  try( left; split; assumption)
+    ).
+
+  (* Eps/Eps case *)
+  left. simpl. trivial.
+  
+Defined.
+
+Definition Dual {t t':protoType} {T T':type} (p1:protoExp T t) (p2:protoExp T' t') : Prop := DualT t t'.
+
+Fixpoint runProto {t t':protoType} {T T':type} (p1:protoExp T t) (p2:protoExp T' t') 
+  : (Dual p1 p2) -> (message T).
+Proof.
+
+       intro pf. destruct p1 (*eqn : p1Val*); destruct p2 (*eqn : p2Val*); try (inversion pf).
+
+       subst. apply (runProto _ _ _ _ p1 (p m)). unfold Dual. assumption.
+       subst. apply (runProto _ _ _ _ (p m) p2). unfold Dual. assumption.
+
+       destruct b.
+       apply (runProto _ _ _ _ p1_1 p2_1 ). unfold Dual. assumption.
+       apply (runProto _ _ _ _ p1_2 p2_2 ). unfold Dual. assumption.
+       
+       destruct b.
+       assert (message R).
+       apply (runProto _ _ _ _ p1_1 p2_1 ). unfold Dual. assumption. exact (leither _ _ X).
+       assert (message S).
+       apply (runProto _ _ _ _ p1_2 p2_2 ). unfold Dual. assumption. exact (reither _ _ X).
+
+       exact m.
+Defined.
+
+(*Definition realType{t:type} (m:message t) : type :=
+  match m with
+  | leither t1 _ _ => t1
+  | reither _ t2 _ => t2
+  | _ => t
+  end.*)
+
+Definition realEither (t:type) (b:bool) : type :=
+  match t with
+  | Either t1 t2 => if b then t1 else t2
+  | _ => t
+  end.
+
+Fixpoint realEither'{t t':protoType} {T T':type}
+           (p1:protoExp T t) (p2:protoExp T' t') : type :=
+  match p1 with
+  | OfferC p1' p1'' =>
+    match p2 with
+    | ChoiceC b p2' p2'' => realEither T b
+    | _ => T
+    end
+  | SendC m p1' =>
+    match p2 with
+    | ReceiveC f => realEither' p1' (f (bad (funType f)))
+    | _ => T
+    end
+  | _ => T
+  end.
+
+Hint Unfold realEither' realEither.
+
+
+Inductive runProtoBigStep : forall (T T':type), forall (t t':protoType) (p1:protoExp T t) (p2:protoExp T' t') (m:message T)(*(realEither' p1 p2))*), Prop :=
+  
+| returnR : forall T T' (m:message T) (m':message T'),
+    runProtoBigStep _ _ _ _ (ReturnC m) (ReturnC m') m
+| sendR : forall X Y Y' p1t p2t
+            (p1':protoExp Y p1t)
+            (f: ((message X) -> (protoExp Y' p2t)))
+            (m:message X) m'(*(m':message (realEither' p1' (f m)))*)
+            ,
+            
+            
+       
+        runProtoBigStep _ _ p1t p2t p1' (f m) m' ->
+        runProtoBigStep _ _ _ _ (SendC m p1') (ReceiveC f) m'
+| receiveR : forall X Y Y' p1t p2t m'
+            (m:message X)
+            (f: ((message X) -> (protoExp Y' p2t)))
+            (p1':protoExp Y p1t),
+            runProtoBigStep _ _ _ _ (f m) p1' m' ->
+            runProtoBigStep _ _ _ _ (ReceiveC f) (SendC m p1') m'
+| choiceRt : forall R R' S S' r r' s s'
+               (r:protoExp R r) (r0:protoExp R' r')
+               (s:protoExp S s) (s0:protoExp S' s')
+               (m:message R) (m':message S),
+    runProtoBigStep _ _ _ _ r r0 m ->
+    runProtoBigStep _ _ _ _ s s0 m' ->
+    runProtoBigStep _ _ _ _ (ChoiceC true r s) (OfferC r0 s0) m
+
+| choiceRf : forall R R' S S' r r' s s'
+               (r:protoExp R r) (r0:protoExp R' r')
+               (s:protoExp S s) (s0:protoExp S' s')
+               (m:message R) (m':message S),
+    runProtoBigStep _ _ _ _ r r0 m ->
+    runProtoBigStep _ _ _ _ s s0 m' ->
+    runProtoBigStep _ _ _ _ (ChoiceC false r s) (OfferC r0 s0) m'
+
+| offerRt : forall R R' S S' r r' s s' m m'
+              (r:protoExp R r) (r0:protoExp R' r')
+              (s:protoExp S s) (s0:protoExp S' s'),
+    runProtoBigStep _ _ _ _ r r0 m ->
+    runProtoBigStep _ _ _ _ s s0 m' ->
+    runProtoBigStep _ _ _ _ (OfferC r s) (ChoiceC true r0 s0) (leither _ _ m) 
+
+| offerRf : forall R R' S S' r r' s s' m m'
+              (r:protoExp R r) (r0:protoExp R' r')
+              (s:protoExp S s) (s0:protoExp S' s'),
+    runProtoBigStep _ _ _ _ r r0 m ->
+    runProtoBigStep _ _ _ _ s s0 m' ->
+    runProtoBigStep _ _ _ _ (OfferC r s) (ChoiceC false r0 s0) (reither _ _ m').
+
+Inductive step : forall (T R T':type), forall (t r t':protoType), (protoExp T t) -> (protoExp R r) -> (protoExp T' t') -> Prop :=
+| ST_Send_Rec : forall X x Y y  mt
+                  (m:message mt) (p1':protoExp X x)
+                  (f:(message mt) -> protoExp Y y),
+    step _ _ _ _ _ _ (SendC m p1') (ReceiveC f) p1'
+| ST_Rec_Send : forall X x Y y mt (m:message mt) (p1':protoExp X x)
+                       (f:(message mt) -> protoExp Y y),                     
+    step _ _ _ _ _ _ (ReceiveC f) (SendC m p1') (f m)
+| ST_Choice_true : forall R R' S S' r r' s s'
+                     (r:protoExp R r) (r0:protoExp R' r')
+                     (s:protoExp S s) (s0:protoExp S' s'),
+    step _ _ _ _ _ _ (ChoiceC true r s) (OfferC r0 s0) r
+| ST_Choice_false : forall R R' S S' r r' s s'
+                     (r:protoExp R r) (r0:protoExp R' r')
+                     (s:protoExp S s) (s0:protoExp S' s'),
+    step _ _ _ _ _ _ (ChoiceC false r s) (OfferC r0 s0) s
+| ST_Offer_true : forall R R' S S' r r' s s'
+                     (r:protoExp R r) (r0:protoExp R' r')
+                     (s:protoExp S s) (s0:protoExp S' s'),
+    step _ _ _ _ _ _ (OfferC r0 s0) (ChoiceC true r s)  r0
+| ST_Offer_false : forall R R' S S' r r' s s'
+                     (r:protoExp R r) (r0:protoExp R' r')
+                     (s:protoExp S s) (s0:protoExp S' s'),
+    step _ _ _ _ _ _ (OfferC r0 s0) (ChoiceC false r s) s0.
+
+Definition proto1 :=
+  send (basic 1);
+  EpsC.
+
+Definition proto2 :=
+  x <- receive;
+  ReturnC (t:=Basic) x.
+
+Notation "'stepe'" := (step _ _ _ _ _ _).
+
+Example stepEx1 : stepe proto1 proto2 EpsC.
+Proof.
+  constructor.
+Qed.
+
+Definition proto3 (b:bool) :=
+  choice b EpsC
+         proto1. Check proto3.
+
+Definition proto4 :=
+  offer EpsC
+        proto2. Check proto4.
+
+Example stepEx2 : stepe (proto3 true) proto4 EpsC.
+Proof.
+  unfold proto3. unfold proto4. constructor.
+Qed.
+
+Example stepEx2' : stepe (proto3 false) proto4 proto1.
+Proof.
+  constructor.
+Qed.
+
+Example stepEx3' : stepe proto4 (proto3 true) EpsC.
+Proof.
+  unfold proto3. unfold proto4. constructor.
+Qed.
+
+Example stepEx3 : stepe proto4 (proto3 false) proto2.
+Proof.
+  constructor.
+Qed.
+           
+Definition relation3 (T R T':type) (t r t':protoType)  :=  (*forall (T R T':type), forall (t r t':protoType),*) (protoExp T t) -> (protoExp R r) -> (protoExp T' t') -> Prop.
+
+Inductive multi : forall (T R T':type), forall (t r t':protoType), (protoExp T t) -> (protoExp R r) -> (protoExp T' t') -> Prop :=
+| multi_refl : forall (T R T':type) (t r t':protoType) (x:protoExp T t) (y:protoExp R r),
+    multi _ _ _ _ _ _ x y x
+| multi_step : forall (T T' R R' S:type) (t t' r r' s:protoType),
+    forall (x:protoExp T t) (x':protoExp T' t')
+      (y:protoExp R r) (y':protoExp R' r')
+      (z:protoExp S s),
+                    step _ _ _ _ _ _ x x' y ->
+                    multi _ _ _ _ _ _ y y' z ->
+                    multi _ _ _ _ _ _ x x' z.
+
+Definition incPayload (m:message Basic) : (message Basic) :=
+  match m with
+  | basic n => basic (n + 1)
+  | _ => basic 0                 
+  end.
+
+Definition proto5 :=
+  send (basic 1);
+  x <- receive;
+  ReturnC (t:=Basic) x.
+
+Definition proto6 :=
+  y <- receive;
+  send (incPayload y);
+  EpsC.
+
+Example multiEx1 : multi _ _ _ _ _ _ proto5 proto6 (ReturnC (basic 2)).
+Proof. Print multi_step. specialize multi_step. intros. apply H with (R:=Basic) (R':=Basic) (r:=(Receive Basic (Eps Basic))) (r':=(Send Basic (Eps Basic))) (y:=  x <- receive; ReturnC (t:=Basic) x) (y':=send (incPayload (basic 1));EpsC). constructor. apply H with (R:=Basic) (R':=Basic) (r:=(Eps Basic)) (r':=(Eps Basic)) (y:= ReturnC (basic 2)) (y':=EpsC). constructor. constructor. exact (Basic). exact (Eps Basic).
+Qed.
+
+Theorem big_multistep_equiv {t t':protoType} {T T':type} {p1:protoExp T t} {p2:protoExp T' t'} : forall m, runProtoBigStep _ _ _ _ p1 p2 m ->
+                         multi _ _ _ _ _ _ p1 p2 (ReturnC m).
+Proof.
+  intros. generalize dependent t'. generalize dependent T'. dependent induction p1; destruct p2; try (intros H; inversion H; contradiction).
+  intros H. dep_destruct H. specialize multi_step. intros H0. apply H0 with (R:=Y) (R':=Y') (r:=p') (r':= p'0) (y:=p1) (y':=p m). constructor. apply IHp1. assumption.
+  intros H0. dep_destruct H0. specialize multi_step. intros H1. apply H1 with (R:=Y') (R':=Y) (r:=p') (r':= p'0) (y:=p m0) (y':=p2). constructor. apply H. assumption.
+
+  intros HH. inversion HH.
+  intros HH. inversion HH.
+  intros HH. inversion HH.
+  intros HH. inversion HH.
+  intros H. dep_destruct H. specialize multi_step. intros H0. apply H0 with (R:=R) (R':=R0) (r:=r) (r':=r0) (y:=p1_1) (y':=p2_1). constructor. apply IHp1_1. assumption.
+  specialize multi_step. intros H0. apply H0 with (R:=S) (R':=S0) (r:=s) (r':=s0) (y:=p1_2) (y':=p2_2). constructor. apply IHp1_2. assumption.
+  
+  intros H. dep_destruct H. specialize multi_step. intros H0. apply H0 with (R:=R) (R':=R0) (r:=r) (r':=r0) (y:=p1_1) (y':=p2_1). constructor. (*apply IHp1_1.*) admit.
+  specialize multi_step. intros H0. apply H0 with (R:=S) (R':=S0) (r:=s) (r':=s0) (y:=p1_2) (y':=p2_2). constructor. (*apply IHp1_2.*) admit.
+
+  intros H. dep_destruct H. constructor. exact (Basic). exact (Eps Basic). Abort. 
+  (*
+  intros H. dep_destruct H. specialize multi_step. intros H0. apply H0 with (R:=R) (R':=R0) (r:=r) (r':=r0) (y:=p1_1) (y':=p2_1). constructor. admit.
+
+  specialize multi_step. intros H0. apply H0 with (R:=Either R S) (R':=R0) (r:=r) (r':=r0) (y:=p1_1) (y':=p2_1). constructor. apply IHp1_1. assumption.
+  specialize multi_step. intros H0. apply H0 with (R:=S) (R':=S0) (r:=s) (r':=s0) (y:=p1_2) (y':=p2_2). constructor. apply IHp1_2. assumption. *)
+
+
+Theorem runProto_iff_multi{t t':protoType} {T T':type} {p1:protoExp T t} {p2:protoExp T' t'}{p:Dual p1 p2} : forall m,
+      ((runProto p1 p2 p) = m) <-> multi _ _ _ _ _ _ p1 p2 (ReturnC m).
+Proof.
+Admitted.
+
+Theorem runProto_iff_bigStep{t t':protoType} {T T':type} {p1:protoExp T t} {p2:protoExp T' t'}{p:Dual p1 p2} : forall m,
+    ((runProto p1 p2 p) = m) <-> runProtoBigStep _ _ _ _ p1 p2 m.
+Proof.
+  intro m.
+  assert (((runProto p1 p2 p) = m) <-> multi _ _ _ _ _ _ p1 p2 (ReturnC m)).
+  apply runProto_iff_multi. Admitted. 
